llvm.checker: integrate improved induction principle

cogent/src/Cogent/LLVM/CoqGen.hs
@@ -86,7 +86,7 @@ data Lit
     deriving (Show)
 
 data Expr
-    = BPrim PrimOp Expr Expr
+    = Prim PrimOp (CoqList Expr)
     | App Expr Expr
     | Unit
     | Lit Lit
@@ -155,7 +155,7 @@ genType t = error $ show t
 
 genExpr :: (Show a, Show b) => FunBodies -> TypedExpr t v a b -> Expr
 genExpr fb (TE _ (C.ILit int p)) = Lit $ genLit int p
-genExpr fb (TE _ (C.Op op [a, b])) = BPrim (genOp (exprType a) op) (genExpr fb a) (genExpr fb b)
+genExpr fb (TE _ (C.Op op os@(a : _))) = Prim (genOp (exprType a) op) (mkCoqList (genExpr fb) os)
 genExpr fb (TE _ (C.Let _ val body)) = Let (genExpr fb val) (genExpr fb body)
 genExpr fb (TE _ (C.Variable (idx, _))) = Var (finInt idx)
 genExpr fb (TE _ C.Unit) = Unit
