cogent/llvm/checker/coq/Cogent.v
@@ -94,7 +94,7 @@ Section Syntax.
     | Var (i : index)
     | Let (e : expr) (b : expr)
     (* | LetBang (is : set index) (e : expr) (b : expr) *)
-    | BPrim (op : prim_op) (a b : expr)
+    | Prim (op : prim_op) (os : list expr)
     | If (c : expr) (b1 : expr) (b2 : expr)
     | Cast (t : num_type) (e : expr)
 
@@ -113,60 +113,74 @@ Section Syntax.
     (* | AFun (funtyp : 'f)  (ts : list type) *)
     .
 
-    Print expr_ind.
+  (* Improved induction principle thanks to @amblafont *)
+  Definition expr_ind' :
 
-    (* I copied and pasted the term printed above, and changed the type so that
-it matches what we want.
-     *)
-
-      Definition expr_ind' :
-    
-      forall P : expr -> Prop,
-       P Unit ->
-       (forall l : lit, P (Lit l)) ->
-       (forall i : index, P (Var i)) ->
-       (forall e : expr, P e -> forall b : expr, P b -> P (Let e b)) ->
-       (forall (op : prim_op) (a : expr), P a -> forall b : expr, P b -> P (BPrim op a b)) ->
-       (forall c : expr, P c -> forall b1 : expr, P b1 -> forall b2 : expr, P b2 -> P (If c b1 b2)) ->
-       (forall (t : num_type) (e : expr), P e -> P (Cast t e)) ->
-       (* in the Struct case, we add the assumption Forall P es *)
-       (forall (ts : list type) (es : list expr), Forall P es -> P (Struct ts es)) ->
-       (forall e : expr, P e -> forall f7 : field, P (Member e f7)) ->
-       (forall e : expr, P e -> forall (f8 : field) (b : expr), P b -> P (Take e f8 b)) ->
-       (forall e : expr, P e -> forall (f9 : field) (v : expr), P v -> P (Put e f9 v)) ->
-       (forall f10 : expr, P f10 -> P (Fun f10)) ->
-       (forall f11 : expr, P f11 -> forall a : expr, P a -> P (App f11 a)) -> forall e : expr, P e :=
-    fun (P : expr -> Prop) (f : P Unit) (f0 : forall l : lit, P (Lit l)) (f1 : forall i : index, P (Var i))
-  (f2 : forall e : expr, P e -> forall b : expr, P b -> P (Let e b))
-  (f3 : forall (op : prim_op) (a : expr), P a -> forall b : expr, P b -> P (BPrim op a b))
-  (f4 : forall c : expr, P c -> forall b1 : expr, P b1 -> forall b2 : expr, P b2 -> P (If c b1 b2))
-  (f5 : forall (t : num_type) (e : expr), P e -> P (Cast t e))
-  (f6 : forall (ts : list type)(es : list expr), Forall P es -> P (Struct ts es))
-  (f7 : forall e : expr, P e -> forall f7 : field, P (Member e f7))
-  (f8 : forall e : expr, P e -> forall (f8 : field) (b : expr), P b -> P (Take e f8 b))
-  (f9 : forall e : expr, P e -> forall (f9 : field) (v : expr), P v -> P (Put e f9 v))
-  (f10 : forall f10 : expr, P f10 -> P (Fun f10))
-  (f11 : forall f11 : expr, P f11 -> forall a : expr, P a -> P (App f11 a)) =>
-fix F (e : expr) : P e :=
-  match e as e0 return (P e0) with
-  | Unit => f
-  | Lit l => f0 l
-  | Var i => f1 i
-  | Let e0 b => f2 e0 (F e0) b (F b)
-  | BPrim op a b => f3 op a (F a) b (F b)
-  | If c b1 b2 => f4 c (F c) b1 (F b1) b2 (F b2)
-  | Cast t e0 => f5 t e0 (F e0)
-  | Struct ts es => f6 ts es
-            (* applying the induction hypothesis requires a proof that Forall P es.
-             This is done by a list recursion *)
-           (list_ind _ (Forall_nil P)   (fun a _ H  =>  Forall_cons a (F a) H) _)
-  | Member e0 f12 => f7 e0 (F e0) f12
-  | Take e0 f12 b => f8 e0 (F e0) f12 b (F b)
-  | Put e0 f12 v => f9 e0 (F e0) f12 v (F v)
-  | Fun f12 => f10 f12 (F f12)
-  | App f12 a => f11 f12 (F f12) a (F a)
-  end.
-
+  forall P : expr -> Prop,
+    P Unit ->
+    (forall l : lit, P (Lit l)) ->
+    (forall i : index, P (Var i)) ->
+    (forall e : expr, P e -> forall b : expr, P b -> P (Let e b)) ->
+    (* in the Prim case, we add the assumption Forall P os *)
+    (forall (op : prim_op) (os : list expr), Forall P os -> P (Prim op os)) ->
+    (forall c : expr, P c -> forall b1 : expr, P b1 -> forall b2 : expr, P b2 -> P (If c b1 b2)) ->
+    (forall (t : num_type) (e : expr), P e -> P (Cast t e)) ->
+    (* in the Struct case, we add the assumption Forall P es *)
+    (forall (ts : list type) (es : list expr), Forall P es -> P (Struct ts es)) ->
+    (forall e : expr, P e -> forall f : field, P (Member e f)) ->
+    (forall e : expr, P e -> forall (f : field) (b : expr), P b -> P (Take e f b)) ->
+    (forall e : expr, P e -> forall (f : field) (v : expr), P v -> P (Put e f v)) ->
+    (forall (ts : tags) (n : name) (e : expr), P e -> P (Con ts n e)) ->
+    (forall (t : type) (e : expr), P e -> P (Promote t e)) ->
+    (forall (ts : tags) (e : expr), P e -> P (Esac ts e)) ->
+    (forall (ts : tags) (e : expr),  P e -> forall (n : name) (b1 : expr), 
+      P b1 -> forall b2 : expr, P b2 -> P (Case ts e n b1 b2)) ->
+    (forall f14 : expr, P f14 -> P (Fun f14)) ->
+    (forall f15 : expr, P f15 -> forall a : expr, P a -> P (App f15 a)) -> forall e : expr,
+      P e :=
+        fun (P : expr -> Prop) (f : P Unit)
+        (f0 : forall l : lit, P (Lit l))
+        (f1 : forall i : index, P (Var i))
+        (f2 : forall e : expr, P e -> forall b : expr, P b -> P (Let e b))
+        (f3 : forall (op : prim_op) (os : list expr), Forall P os -> P (Prim op os))
+        (f4 : forall c : expr, P c -> forall b1 : expr, P b1 -> forall b2 : expr, P b2 -> P (If c b1 b2))
+        (f5 : forall (t : num_type) (e : expr), P e -> P (Cast t e))
+        (f6 : forall (ts : list type) (es : list expr), Forall P es -> P (Struct ts es))
+        (f7 : forall e : expr, P e -> forall f : field, P (Member e f))
+        (f8 : forall e : expr, P e -> forall (f : field) (b : expr), P b -> P (Take e f b))
+        (f9 : forall e : expr, P e -> forall (f : field) (v : expr), P v -> P (Put e f v))
+        (f10 : forall (ts : tags) (n : name) (e : expr), P e -> P (Con ts n e))
+        (f11 : forall (t : type) (e : expr), P e -> P (Promote t e))
+        (f12 : forall (ts : tags) (e : expr), P e -> P (Esac ts e))
+        (f13 : forall (ts : tags) (e : expr), P e -> forall (n : name) (b1 : expr),
+          P b1 -> forall b2 : expr, P b2 -> P (Case ts e n b1 b2))
+        (f14 : forall f14 : expr, P f14 -> P (Fun f14))
+        (f15 : forall f15 : expr, P f15 -> forall a : expr, P a -> P (App f15 a)) =>
+          fix F (e : expr) : P e :=
+            match e as e0 return (P e0) with
+            | Unit => f
+            | Lit l => f0 l
+            | Var i => f1 i
+            | Let e0 b => f2 e0 (F e0) b (F b)
+            | Prim op os => f3 op os
+                (* applying the induction hypothesis requires a proof that Forall P os.
+                This is done by a list recursion *)
+                (list_ind _ (Forall_nil P) (fun a _ H => Forall_cons a (F a) H) _)
+            | If c b1 b2 => f4 c (F c) b1 (F b1) b2 (F b2)
+            | Cast t e0 => f5 t e0 (F e0)
+            | Struct ts es => f6 ts es
+                (* as above *)
+                (list_ind _ (Forall_nil P) (fun a _ H => Forall_cons a (F a) H) _)
+            | Member e0 f12 => f7 e0 (F e0) f12
+            | Take e0 f12 b => f8 e0 (F e0) f12 b (F b)
+            | Put e0 f12 v => f9 e0 (F e0) f12 v (F v)
+            | Con ts n e0 => f10 ts n e0 (F e0)
+            | Promote t e0 => f11 t e0 (F e0)
+            | Esac ts e0 => f12 ts e0 (F e0)
+            | Case ts e0 n b1 b2 => f13 ts e0 (F e0) n b1 (F b1) b2 (F b2)
+            | Fun f16 => f14 f16 (F f16)
+            | App f16 a => f15 f16 (F f16) a (F a)
+            end.
 
   Variant def : Type :=
     | FunDef (n : name) (t : type) (rt : type) (b : expr).
